theories/ITree/Logic/AF.v
@@ -1,0 +1,470 @@
+From Coq Require Import
+  Basics
+  Classes.Morphisms.
+
+From Coinduction Require Import
+  coinduction lattice.
+
+From ExtLib Require Import
+  Structures.Monad
+  Data.Monads.StateMonad.
+
+From CTree Require Import
+  Events.Core
+  ITree.Core
+  ITree.Pred
+  ITree.Equ  
+  ITree.Logic.Trans
+  ITree.Logic.CanStep
+  ITree.Events.Writer
+  Logic.Ctl
+  Logic.Kripke.
+
+Set Implicit Arguments.
+Generalizable All Variables.
+
+Import ITreeNotations CtlNotations.
+Local Open Scope ctl_scope.
+Local Open Scope itree_scope.
+  
+(*| CTL logic lemmas on c/itrees |*)
+Section CtlITrees.
+  Context {E: Type} {HE: Encode E} {X: Type}
+    (φ: itree E X -> World E -> Prop) {HP: Proper (equ X ==> eq ==> iff) φ}.
+  
+  (*| [t |= AF φ] is semantic and requires double induction, on [AF] and inside it, in
+  [ktrans]. Attempt to simplify to one induction with [AFInd] |*)
+  Inductive AFInd: itree E X -> World E -> Prop :=
+  | AFIndBase: forall (t: itree E X) (w: World E),
+      φ t w ->
+      AFInd t w
+  | AFIndDoneBase: forall t (x: X),
+      observe t = RetF x ->
+      φ Itree.stuck (Done x) ->
+      AFInd t Pure
+  | AFIndFinishBase: forall t (e: E) (v: encode e) (x: X),
+      observe t = RetF x ->
+      φ Itree.stuck (Finish e v x) ->
+      AFInd t (Obs e v)
+  | AFIndTau: forall t u w,
+      observe t = TauF u ->
+      AFInd u w ->
+      AFInd t w
+  |AFIndVis: forall (t: itree E X) w e k (_: encode e),
+      observe t = VisF e k ->
+      not_done w ->
+      (forall (v: encode e), AFInd (k v) (Obs e v)) ->
+      AFInd t w.
+
+  Lemma af_ind_stuck_done: forall (x: X),
+    AFInd Itree.stuck (Done x) <->
+    φ Itree.stuck (Done x).
+  Proof.
+    split; intros.
+    - dependent induction H; auto.
+    - now apply AFIndBase.
+  Qed.
+
+  Lemma af_ind_stuck_finish: forall (e: E) (v: encode e) (x: X),
+    AFInd Itree.stuck (Finish e v x) <->
+    φ Itree.stuck (Finish e v x).
+  Proof.
+    split; intros.
+    - dependent induction H; auto.
+    - now apply AFIndBase.
+  Qed.
+
+  Lemma af_afind {Hpr: @Productive E HE}
+                 {TauInv: forall (t: itree E X) w, φ t w  -> φ (Tau t) w}
+    : forall (t: itree E X) (w: World E),
+      AFInd t w <-> cau true (fun _ _ => True) φ t w.
+  Proof.
+    split; intros; induction H.
+    (* -> *)
+    - now apply MatchA.
+    - apply StepA; auto; split.
+      + exists Itree.stuck, (Done x).
+        Opaque Itree.stuck.
+        cbn. rewrite H.
+        apply KtransDone; auto.
+      + intros t' w' TR.
+        ktrans_ind TR.
+        * rewrite H in x1; inv x1.
+        * rewrite H in x1; inv x1.
+        * rewrite H in x2; inv x2.          
+          observe_equ x.
+          rewrite <- Eqt, H1.          
+          now apply MatchA.
+    - apply StepA; auto; split.
+      + exists Itree.stuck, (Finish e v x).
+        Opaque Itree.stuck.
+        cbn. rewrite H.
+        apply KtransFinish; auto.
+      + intros t' w' TR.
+        ktrans_ind TR.
+        * rewrite H in x1; inv x1.
+        * rewrite H in x1; inv x1.
+        * rewrite H in x2; inv x2.          
+          observe_equ x.
+          rewrite <- Eqt, H1.          
+          now apply MatchA.
+    - observe_equ H.
+      rewrite Eqt; clear Eqt.
+      destruct IHAFInd.
+      + apply MatchA.
+        (* TauInv here *)
+        now apply TauInv.
+      + destruct H2.
+        apply StepA; auto.
+        split; auto with ctl.
+        intros t' w' TR.
+        apply H3.
+        now rewrite ktrans_tau in TR.
+    - observe_equ H.
+      rewrite Eqt; clear Eqt.
+      apply StepA; auto; split; auto with ctl.
+      intros t' w' TR.
+      + apply ktrans_vis in TR as (v & ? & -> & ?).
+        rewrite H3.
+        eapply H2.
+    - (* <- *)
+      now apply AFIndBase.
+    - destruct H0, H1; clear H H1.
+      destruct H0 as (t' & w' & TR).
+      cbn in TR.
+      dependent induction TR.
+      + observe_equ x.
+        eapply AFIndVis with (e:=e) (k:=k); auto.
+        intros v'.
+        apply H3; cbn.
+        rewrite <- x0.
+        apply KtransObs; auto.
+      + eapply AFIndTau with (u:=t0); auto.
+        eapply (IHTR HP) with (t':=t'); auto.
+        -- intros t_ w_ TR_.
+           apply H2; cbn.
+           rewrite <- x0.
+           now apply ktrans_tau.
+        -- intros t_ w_ TR_.
+           apply H3; cbn.
+           rewrite <- x0.
+           now apply ktrans_tau.
+      + apply AFIndDoneBase with (x:=x0); auto.
+        assert (TR_: [t, Pure] ↦ [Itree.stuck, Done x0]).
+        { cbn; rewrite <- x1; apply KtransDone; auto. }
+        specialize (H3 _ _ TR_).
+        now apply af_ind_stuck_done.
+      + apply AFIndFinishBase with (x:=x0); auto.
+        assert (TR_: [t, Obs e v] ↦ [Itree.stuck, Finish e v x0]).
+        { cbn; rewrite <- x1; apply KtransFinish; auto. }
+        specialize (H3 _ _ TR_).
+        now apply af_ind_stuck_finish.
+  Qed.
+  
+  Lemma ctl_af_tau: forall (t: itree E X) w φ,
+      <( t, w |= AF now φ )> -> 
+      <( {Tau t}, w |= AF (now φ) )>.
+  Proof.
+    intros.
+    unfold entailsF in H.
+    induction H.
+    - now next; left.
+    - Opaque entailsF.
+      destruct H0, H1; clear H H1.
+      destruct H0 as (t' & w' & TR).
+      specialize (H3 _ _ TR); cbn in H3.
+      next; right.
+      split.
+      * apply can_step_tau.
+        exists t', w'; auto.
+      * intros t_ w_ TR_.
+        rewrite ktrans_tau in TR_.
+        now apply H2.
+  Qed.
+
+  Lemma ctl_af_vis: forall (e: E) (k: encode e -> itree E X) (_: encode e) w φ,
+      (φ w \/ (not_done w /\ forall (x: encode e), <( {k x}, {Obs e x} |= AF now φ )>)) ->
+      <( {Vis e k}, w |= AF now φ )>.        
+  Proof.
+    intros.
+    destruct H as [H | [Hd H]].
+    - now next; left.
+    - next; right; next; split.
+      + now apply can_step_vis.
+      + intros t' w' TR'.
+        apply ktrans_vis in TR' as (? & -> & -> & ?).
+        apply H.
+  Qed.
+
+End CtlITrees.
+
+Section CtlAfBind.
+  Context {E: Type} {HE: Encode E}.
+
+  Lemma ctl_stuck_obs_af{X}: forall (x: X) φ w,
+      return_eq X x w ->
+      ~ <( {Itree.stuck: itree E X}, w |= AF obs φ )>.
+  Proof.
+    intros * Hret Hcontra.
+    inv Hcontra.
+    - inv H; cbn in *; subst. 
+      destruct Hret; inv H.
+    - destruct H0 as ((? & ? & ?) & ?).
+      now apply ktrans_stuck in H0.
+  Qed.
+
+  Lemma ctl_obs_af_inv{X}: forall (t: itree E X) φ w,
+      <( t, w |= AF obs φ )> ->
+      not_done w.  
+  Proof.
+    intros * Haf.
+    next in Haf; destruct Haf; cbn in H.
+    - inv H. 
+      constructor.
+    - destruct H. 
+      destruct H as (t' & w' & TR).
+      now eapply ktrans_not_done with t t' w'.
+  Qed.
+  Hint Resolve ctl_obs_af_inv: ctl.
+
+  Theorem ctl_bind_af_l{X Y}: forall (t: itree E Y) (k: Y -> itree E X) φ w,
+      <( t, w |= AF obs φ )> ->
+      <( {x <- t ;; k x}, w |= AF obs φ )>.
+  Proof.
+    intros * Haf.
+    revert X k.
+    induction Haf; intros; subst. 
+    - (* MatchA *)
+      next; left; cbn.
+      apply H.
+    - (* StepA *)
+      destruct H0, H1; clear H H0.
+      destruct H1 as (te & we & TR); cbn in TR.
+      dependent destruction TR.
+      + next; right; next; split. 
+        * apply can_step_bind_l with t0 (Obs e v); cbn. 
+          -- rewrite <- x0.
+             now apply KtransObs.
+          -- constructor.
+        * intros k' w' TR'.
+          apply ktrans_bind_inv in TR'
+              as [(t' & TR' & Hd & ?) |
+               [(y & TRr & -> & TRk) |
+                 (e' & v' & x' & TRr & -> & TRk)]].
+          -- rewrite H1.
+             apply (H3 t' w' TR').
+          -- specialize (H2 Itree.stuck (Done y) TRr).
+             Transparent entailsF.
+             apply ctl_stuck_obs_af with (x:=y) in H2; intuition.
+          -- specialize (H2 Itree.stuck (Finish e' v' x') TRr).
+             apply ctl_stuck_obs_af with (x:=x') in H2; intuition.
+      + observe_equ x0.
+        rewrite Eqt.
+        assert (TRtau: ktrans_ (observe t) w (observe t') we).
+        { rewrite x0; now apply KtransTau. }        
+        next; right; next; split. 
+        * eapply can_step_bind_l; cbn.
+          apply KtransTau; eauto.
+          specialize (H3 t' we TRtau _ k); cbn in H3.        
+          now apply ctl_obs_af_inv in H3.
+        * intros k' w' TR'.
+          apply ktrans_bind_inv in TR'
+              as [(t_ & TR_ & Hd & ?) |
+                   [(y & TRt' & -> & TRk) |
+                     (e' & v' & x' & TRr & -> & TRk)]].
+          -- rewrite H.
+             specialize (H3 t_ w'); cbn in H2.
+             rewrite ktrans_tau in TR_.
+             apply H3; cbn.
+             rewrite x0.
+             now apply ktrans_tau.
+          -- cbn in TRt'.
+             rewrite <- x0 in TRt'.
+             specialize (H2 Itree.stuck (Done y) TRt'); cbn in H2.             
+             Transparent entailsF.
+             eapply ctl_stuck_obs_af with (x:=y) in H2; intuition.
+          -- cbn in TRr.
+             rewrite <- x0 in TRr.
+             specialize (H2 Itree.stuck (Finish e' v' x') TRr); cbn in H2.             
+             Transparent entailsF.
+             eapply ctl_stuck_obs_af with (x:=x') in H2; intuition.
+      + assert (TRt: ktrans_ (observe t) Pure (observe Itree.stuck) (Done x0)).
+        { rewrite <- x1; apply KtransDone; reflexivity. }.
+        specialize (H3 Itree.stuck (Done x0) TRt _ k); cbn in H3.
+        apply ctl_obs_af_inv in H3; inv H3.
+      + assert (TRt: ktrans_ (observe t) (Obs e v) (observe Itree.stuck) (Finish e v x0)).
+        { rewrite <- x1; apply KtransFinish; reflexivity. }.
+        specialize (H3 Itree.stuck (Finish e v x0) TRt _ k).
+        apply ctl_obs_af_inv in H3; inv H3.
+  Qed.
+
+  Lemma ctl_return_af_inv{X}: forall (t: itree E X) w (r: X),
+      <( t, w |= AF return r )> ->
+      return_eq X r w \/ ALeaf (eq r) t.
+  Proof.
+    intros.
+    induction H.
+    - left; auto.
+    - destruct H0, H1; clear H H1.
+      destruct H0 as (t' & w' & TR'); cbn.
+      generalize dependent r.      
+      ktrans_ind TR'; intros.
+      + right; eapply ALeafVis.
+        * now rewrite x0.
+        * intro x'.          
+          assert (TR_: [t, w] ↦ [k x', Obs e x']).
+          { cbn.
+            rewrite <- x0.
+            eapply KtransObs; auto.
+          }.
+          destruct (H3 _ _ TR_); cbn in H1.
+          -- destruct H1; inv H1.
+          -- auto.
+      + edestruct IHTR' with (t':=t'); eauto.
+          -- intros t_ w_ TR_.
+             apply H2; cbn.
+             rewrite <- x0; now apply KtransTau.
+          -- intros t_ w_ TR_.
+             apply H3; cbn.
+             rewrite <- x0; now apply KtransTau.
+          -- right.
+             eapply ALeafTau.
+             ++ now rewrite x0.
+             ++ auto.
+      + right; eapply ALeafRet.
+        assert (TR_: [t, Pure] ↦ [Itree.stuck, Done x0]).
+        { cbn.
+          rewrite <- x1.
+          replace (TauF Itree.stuck) with (observe Itree.stuck (X:=X)) by reflexivity.
+          apply KtransDone; auto.
+        }
+        destruct (H3 _ _ TR_); cbn in H0.
+        * destruct H0; dependent destruction H0.
+          now rewrite x1.
+        * now apply ALeaf_stuck in H0.
+        * reflexivity.
+      + right; eapply ALeafRet.
+        assert (TR_: [t, Obs e v] ↦ [Itree.stuck, Finish e v x0]).
+        { cbn.
+          rewrite <- x1.
+          replace (TauF Itree.stuck) with (observe Itree.stuck (X:=X)) by reflexivity.
+          apply KtransFinish; auto.
+        }
+        destruct (H3 _ _ TR_); cbn in H0.        
+        * destruct H0; dependent destruction H0.
+          now rewrite x1.
+        * now apply ALeaf_stuck in H0.
+        * reflexivity.
+  Qed.
+
+  Lemma can_step_bind_r{X Y} {HP: Productive E}:
+    forall (t: itree E Y) (k: Y -> itree E X) w (r: Y),      
+      <( t, w |= AF return r )> ->
+      can_step (k r) w ->
+      can_step (x <- t ;; k x) w.
+  Proof.    
+    intros.
+    apply ctl_return_af_inv in H as [H|H].
+    - destruct H; inv H. (* (kr, w) can step, so w != done *)
+      + apply can_step_not_done in H0; inv H0.
+      + apply can_step_not_done in H0; inv H0. 
+    - revert w k H0.
+      dependent induction H; intros;
+        observe_equ H; rewrite Eqt, ?bind_ret_l; subst.
+      + exact H1.
+      + rewrite bind_tau.
+        eapply can_step_tau.
+        now apply IHALeaf.
+      + rewrite bind_vis.
+        apply can_step_vis.
+        * (* Indeed, [x <- Vis (e: void) ;; k x]
+             does not step, need [Productive E] *)
+          apply HP.
+        * now apply can_step_not_done in H2. 
+  Qed.
+  Hint Resolve can_step_bind_r: ctl.
+
+   Theorem ctl_bind_af_finish{X Y} {HP: Productive E}:
+    forall (t: itree E Y) (k: Y -> itree E X) w φ R,
+      <( t, w |= AF finish R )> ->
+      (forall (e: E) (v: encode e) (y: Y), R e v y -> <( {k y}, {Obs e v} |= AF now φ )>) ->
+      <( {x <- t ;; k x}, w |= AF now φ )>.
+  Proof.
+    intros.
+    revert H0.
+    generalize dependent φ.
+    generalize dependent k.
+    induction H; intros; cbn in H.
+    - inv H.
+     
+    - destruct H0, H1; clear H H1.
+      destruct H0 as (t' & w' & TR'); cbn.
+      generalize dependent r.      
+      ktrans_ind TR'; intros.
+      
+    apply ctl_return_af_inv in H as [H|H].
+    - specialize (H0 w).
+      destruct H; inv H; inv H0.
+      + now next; left.
+      + destruct H1.
+        apply can_step_not_done in H0; inv H0. 
+      + now next; left.
+      + destruct H1.
+        apply can_step_not_done in H0; inv H0.
+    - generalize dependent w.
+      revert H0.
+      dependent induction H; intros; observe_equ H.
+      + now rewrite Eqt, bind_ret_l.
+      + rewrite Eqt, bind_tau.
+        apply ctl_af_tau.
+        now apply IHALeaf.
+      + rewrite Eqt, bind_vis.
+        apply ctl_af_vis.
+        * apply HP.
+        * destruct (not_done_dec w).
+          -- right; split; auto.
+          -- left.
+             specialize (H2 w).
+             auto.
+             apply H1.
+             (* Here, AF [return r] says nothing about the return value
+                of [w], need a more specific predicate like [finish ψ] (see slack) *)
+             apply H1.
+  Admitted.
+  
+  Theorem ctl_bind_af_r{X Y} {HP: Productive E}:
+    forall (t: itree E Y) (k: Y -> itree E X) w φ
+      (ψ: forall (e: E), encode e -> Y -> Prop),
+      <( {(t, w)} |= AF finish ψ )> ->
+      (forall (e: E) (v: encode e) (r: Y),
+          ψ e v r -> <( {(k r, Obs e v)} |= AF now φ )>) ->
+      <( {(x <- t ;; k x, w)} |= AF now φ )>.
+  Proof.
+    intros.
+    apply ctl_return_af_inv in H as [H|H].
+    - inv H; inv H0.
+      + now next; left.
+      + destruct H1.
+        apply can_step_not_done in H0; inv H0. 
+      + now next; left.
+      + destruct H1.
+        apply can_step_not_done in H0; inv H0.
+    - generalize dependent w.
+      dependent induction H; intros; observe_equ H.
+      + now rewrite Eqt, bind_ret_l.
+      + rewrite Eqt, bind_tau.
+        apply ctl_af_tau.
+        now apply IHALeaf.
+      + rewrite Eqt, bind_vis.
+        apply ctl_af_vis.
+        * apply HP.
+        * destruct (not_done_dec w).
+          -- right; split; auto.
+             intro x'.
+             apply H1.
+             (* Here, AF [return r] says nothing about the return value
+                of [w], need a more specific predicate like [finish ψ] (see slack) *)
+             apply H1.
+  Admitted.
+
+End CtlITrees.
