theories/Utils/Utils.v
@@ -91,6 +91,9 @@ Ltac _apply f :=
 (* A smarter version of this should be part of the [coinduction] library *)
 Ltac step_ :=
   match goal with
+  | |- gfp ?b ?x ?y ?z ?v => apply (proj2 (gfp_fp b x y z v)); cbn
+  | |- body (t ?b) ?R ?x ?y ?z ?v => apply (bt_t b R x y z v)
+  | |- body (body (T ?b) ?f) ?R ?x ?y ?z ?v => apply (bT_T b f R x y z v)
   | |- gfp ?b ?x ?y ?z => apply (proj2 (gfp_fp b x y z)); cbn
   | |- body (t ?b) ?R ?x ?y ?z => apply (bt_t b R x y z)
   | |- body (body (T ?b) ?f) ?R ?x ?y ?z => apply (bT_T b f R x y z)
@@ -107,6 +110,8 @@ Ltac step := first [step_ | red; step_].
 
 Ltac step_in H :=
   match type of H with
+  | gfp ?b ?x ?y ?z ?v => apply (gfp_fp b x y z v) in H
+  | body (t ?b) ?R ?x ?y ?z ?v => apply (bt_t b R x y z v) in H
   | gfp ?b ?x ?y ?z => apply (gfp_fp b x y z) in H
   | body (t ?b) ?R ?x ?y ?z => apply (bt_t b R x y z) in H
   | gfp ?b ?x ?y => apply (gfp_fp b x y) in H
